Updating repository to reflect the new developments of this work

analyses/npp_srciror/reference/npp_vars.c
@@ -1,0 +1,36 @@
+#include <stdbool.h>
+
+#define NUM 100
+
+// TIME
+int TIME = 0;
+
+// inputs
+bool the_reset_button = false;
+bool old_the_reset_button = false;
+
+bool the_blockage_button = false;
+bool old_the_blockage_button = false;
+
+int the_water_pressure = 0;
+int old_the_water_pressure = 0;
+
+// outputs
+int the_safety_injection_mode = 1;
+bool the_overridden_mode = false;
+int the_pressure_mode = 1;
+int old_the_pressure_mode = 1;
+
+void reset() {
+    TIME = 0;
+    the_reset_button = false;
+	old_the_reset_button = false;
+	the_blockage_button = false;
+	old_the_blockage_button = false;
+	the_water_pressure = 0;
+	old_the_water_pressure = 0;
+    the_safety_injection_mode = 1;
+	the_overridden_mode = false;
+	the_pressure_mode = 1;
+	old_the_pressure_mode = 1;
+}
