analyses/tis_srciror/renamer.java
@@ -1,0 +1,108 @@
+import java.io.File;
+import java.io.FileNotFoundException;
+import java.io.FileOutputStream;
+import java.io.IOException;
+import java.util.Scanner;
+
+public class renamer {
+	
+	private static String FILE_CONTENT = "";
+	private static int MUTANTS = 975;
+
+	public static void renameMutants(String example) {
+		File[] mutantFiles = new File("mutants/").listFiles();
+		int length = mutantFiles.length;
+
+		boolean alreadyRan = false;
+		for (int i=0; i<length; i++) {
+			if (mutantFiles[i].getName().equals(example + "1.c")) {
+				alreadyRan = true;
+				break;
+			}
+		}
+
+		if (alreadyRan) {
+			return;
+		}
+
+		int k = 1;
+		for (int i=0; i<length; i++) {
+			if (!mutantFiles[i].isHidden() &&
+					!mutantFiles[i].getName().equals("mutateSRC.sh") &&
+					!mutantFiles[i].getName().equals(example + ".c") ) {
+				File oldFile = new File("mutants/" + mutantFiles[i].getName());
+				File newFile = new File("mutants/" + example + k + ".c");
+				oldFile.renameTo(newFile);
+				k++;
+			}
+		}
+	}
+
+	public static void createMainFiles(String example) {
+		readFile("main.c");
+
+		for (int i=1; i<=MUTANTS; i++) {
+			String content = FILE_CONTENT.toString();
+			content = content.replace("#include \"reference/" + example + ".c\"",
+									  "#include \"mutants/" + example + i + ".c\"");
+
+			writeFile(content, "main" + i + ".c");
+		}
+	}
+
+	public static void createRun() {
+		StringBuffer buffer = new StringBuffer();
+		buffer.append("find . -name \"output.txt\" -exec rm -rf {} \\;\n");
+		buffer.append("date +%s ;");
+
+		for (int i=1; i<=MUTANTS; i++) {
+			buffer.append("gcc main" + i + ".c -o main" + i + ";\n");
+		}
+		for (int i=1; i<=MUTANTS; i++) {
+			buffer.append("./main" + i + " >> output.txt\n");
+		}
+		buffer.append("date +%s ;");
+
+		String content = buffer.toString();
+		writeFile(content, "run.sh");
+	}
+
+	public static void readFile(String filename) {
+		try {
+			File file = new File(filename);
+			Scanner s = new Scanner(file);
+			StringBuffer buffer = new StringBuffer();
+
+			String line = "";			
+			while (s.hasNextLine()) {
+				line = s.nextLine();
+				buffer.append(line + "\n");
+			}
+
+			FILE_CONTENT = buffer.toString();
+		} catch (FileNotFoundException e) {
+			e.printStackTrace();
+		}		
+	}
+
+	public static void writeFile(String content, String filename) {
+		try {
+			FileOutputStream fos = new FileOutputStream(filename);
+			fos.write(content.getBytes());
+			fos.close();
+		} catch (FileNotFoundException e) {
+			e.printStackTrace();
+		} catch (IOException e) {
+			e.printStackTrace();
+		}
+	}	
+	
+	public static void main(String[] args) {
+		String example = "tis";
+		//renameTCs(example);
+		renameMutants(example);
+		createMainFiles(example);
+		createRun();
+	}
+
+}
