run/indentify_mutations.py
@@ -1,0 +1,60 @@
+#!/usr/bin/env python
+# -*- coding: utf-8 -*-
+
+from itertools import izip
+from subprocess import call, Popen, PIPE
+import glob
+import csv
+
+srcirorPath = "/home/igormeira/Documents/Git/srciror"
+example = "vm"
+numberOfMutants = 287
+
+# Compare reference with mutations
+# Get line diff
+def mutations(baseFile, mutantFile):
+    lineN = 0
+    with open(baseFile) as base, open(mutantFile) as mutant:
+        for lineB, lineM in izip(base, mutant):
+            lineB = lineB.strip()
+            lineM = lineM.strip()
+            lineN += 1
+            if (lineB != lineM) and (lineB != "") and (lineM != ""):
+                mutation = [lineN, lineB, lineM]
+                return mutation
+    base.close()
+    mutant.close()
+
+def generateCSV(csvData):
+    fileName = "%s_mutation_analyses.csv" %(example)
+
+    with open("%s_mutation_analyses.csv" % (example), 'w') as csvFile:
+        writer = csv.writer(csvFile)
+        writer.writerows(csvData)
+    csvFile.close()
+
+def run():
+    csvData = [["Line Number", "Base File", "Mutated File"]]
+    baseFile = srcirorPath + "/%s_srciror/mutants/%s.c" %(example, example)
+    for n in range(1, numberOfMutants + 1):
+        mutantFile = srcirorPath + "/%s_srciror/mutants/%s%d.c" %(example, example, n)
+        mutation = mutations(baseFile, mutantFile)
+        csvData.append(mutation)
+    generateCSV(csvData)
+
+run()
+
+# Run with equivalent mutants
+def runEquiv():
+    baseFile = srcirorPath + "/%s_srciror/mutants/%s.c" %(example, example)
+    file = open(baseFile, "r")
+    content = file.read()
+    for n in range(1, numberOfMutants + 1):
+        mutantFile = srcirorPath + "/%s_srciror/mutants/%s%d.c" %(example, example, n)
+        fm = open(mutantFile, "w")
+        fm.write(content)
+        print("DONE: %s" %(mutantFile))
+    call("./run.sh", cwd="%s/%s_srciror/" %
+                             (srcirorPath, example), shell=True, stdout=PIPE)
+
+#runEquiv()
