run/run_samples.py
@@ -1,0 +1,156 @@
+#!/usr/bin/env python
+# -*- coding: utf-8 -*-
+
+from subprocess import call, Popen, PIPE
+import datetime
+
+def write_samples_file(exampleName, file_name, samplesNumber):
+    path = "../src/examples/%s/%s" % (exampleName, file_name)
+    file = open(path, 'w')
+    file.write(
+        "Require Import " + exampleName + "_tests.\n" +
+        "Require Import qc_instances.\n\n"
+    )
+
+    text = ""
+    sampleLine = ""
+
+    if exampleName == "vm":
+        sampleLine = "Sample (genValidTrace vm_initial_state VM_s_dfrs vm_possibilities 600).\n"
+    #elif (exampleName == "npp") or (exampleName == "tis"):
+    #    sampleLine = "Sample (genValidTrace %s_initial_state %s_s_dfrs %s_possibilities 500).\n" % (exampleName, exampleName, exampleName)        
+    else:
+        sampleLine = "Sample (genValidTrace %s_initial_state %s_s_dfrs %s_possibilities 600).\n" % (
+            exampleName, exampleName, exampleName)
+
+    for i in range(0, samplesNumber):
+        text = text + sampleLine
+    file.write(text)
+
+
+def getTime(begin, end):
+    formatted_time_begin = float(begin.strftime('%S.%f'))
+    formatted_time_end = float(end.strftime('%S.%f'))
+    formatted_time_begin = formatted_time_begin + (begin.minute * 60.00)
+    formatted_time_end = formatted_time_end + (end.minute * 60.00)
+    return round((formatted_time_end - formatted_time_begin), 2)
+
+
+def getTraces(data):
+    begin_traces = "[["
+    end_traces = "]]"
+    allTraces = []
+    for line in data:
+        if (line is not None):
+            if ("QuickChecking" in line):
+                samples = line.split("QuickChecking")
+                #print(samples)
+                for s in samples:
+                    if (begin_traces in s):
+                        begin = s.find(begin_traces)
+                        #print(begin)
+                        end = s.find(end_traces)
+                        #print(end)
+                        traces = s[begin: end+2]
+                        allTraces.append(traces)
+    #print(allTraces)
+    print(len(allTraces))
+    finalTraces = []
+    for traces in allTraces:
+        count = 0
+        begin = 0
+        end = 0
+        ts_aux = traces[1: len(traces)-1]
+        first = True
+        i = 0
+        while i < len(ts_aux):
+            if first:
+                begin = i
+            if count != 0 or first:
+                first = False
+                if ts_aux[i] == "[":
+                    count = count + 1
+                if ts_aux[i] == "]":
+                    count = count - 1
+            if count == 0:
+                end = i
+                finalTraces.append(ts_aux[begin:end+1])
+                i = i+2
+                first = True
+            i = i+1
+    #print((finalTraces))
+    return finalTraces
+
+
+def is_valid_end(trace):
+    sub_str = trace[-9:-1]
+    if ("REQ" not in sub_str) and (trace != "") and (trace != "[") and (trace != "[]"):
+        return True
+    else:
+        return False
+
+
+def getValidTraces(traces):
+    t = ""
+    validated = []
+    for trace in traces:
+        if trace == traces[-1]:
+            t = trace[0: len(trace)-1]
+        else:
+            t = trace[0: len(trace)]
+        if is_valid_end(t):
+            validated.append(t)
+    print("Traces : %d" % (len(traces)))
+    print("Validos: %d" % (len(validated)))
+    rate = (float(len(validated)) / float(len(traces))) * 100.00
+    print("Rate: %.2f" % (rate))
+    return (validated, round(rate, 2))
+
+
+def compile_samples(exampleName, file_name, rep, samplesNumber):
+    pathDotV = "../src/examples/%s/" % (exampleName)
+    pathOutputs = "../src/examples/%s/Outputs/" % (exampleName)
+
+    write_samples_file(exampleName, file_name, samplesNumber)
+    cmd = "coqc -R ../../ dfrs %s_samples.v" % (exampleName)
+    response = Popen(cmd, cwd=pathDotV, shell=True, stdout=PIPE)
+
+    data = response.communicate()
+    traces = getTraces(data)
+    validTraces = getValidTraces(traces)
+
+    text = ""
+    for vt in validTraces[0]:
+        text = text + vt + " END-TRACE \n\n"
+    outputName = "%s_%d_samples_output_%d.txt" % (exampleName, samplesNumber, rep)
+    cmd = "touch " + outputName
+    call(cmd, cwd=pathOutputs, shell=True)
+    file = open(pathOutputs + outputName, 'w')
+    file.write(text)
+
+    return validTraces[1]
+
+
+def create_file(exampleName):
+    pathDotV = "../src/examples/%s/" % (exampleName)
+    fileName = exampleName + "_" + "samples.v"
+    cmd = "touch " + fileName
+    call(cmd, cwd=pathDotV, shell=True)
+
+    return fileName
+
+
+def runSamples(exampleName, samplesNumber, replicationNumber):
+    fileName = create_file(exampleName)
+    analyses = []
+
+    for rep in range(1, replicationNumber + 1):
+        print("Start %s with %d samples - Rep.: %d") % (exampleName, samplesNumber, rep)
+        begin = datetime.datetime.now().time()
+        rate = compile_samples(exampleName, fileName, rep, samplesNumber)
+        end = datetime.datetime.now().time()
+        time = getTime(begin, end)
+        print("Time: %f \n------------------------" % (time))
+        analyses.append([exampleName, samplesNumber, rep, time, rate])
+    
+    return analyses
