run/tisCSV.py
@@ -1,0 +1,63 @@
+#!/usr/bin/env python
+# -*- coding: utf-8 -*-
+
+def generate_table_data(trace):
+    table = [["Time", "I: the_voltage", "I: the_turn_indicator_lever", "I: the_emergency_flashing", "O: the_indication_lights", "O: the_flashing_mode", "O: the_flashing_timer"],
+             ["0", "0", "0", "0", "2", "2", "0"]]
+    trs = trace.split("[(")
+    time = 0
+    tvoValue = "0"
+    ttilValue = "0"
+    tefValue = "0"
+    tilValue = "2"
+    tfmValue = "2"
+    tftValue = "0"
+    for index, t in enumerate(trs):
+        if "the_voltage" in t:
+            time = time + 1
+            trbBegin = t.find("the_voltage, i ")
+            trbEnd = t.find("); (the_turn_indicator_lever")
+            tvoValue = t[trbBegin+15:trbEnd]
+            if "the_turn_indicator_lever" in t:
+                tbbBegin = t.find("the_turn_indicator_lever, i ")
+                tbbEnd = t.find("); (the_emergency_flashing")
+                ttilValue = t[tbbBegin+28:tbbEnd]
+            if "the_emergency_flashing" in t:
+                twpBegin = t.find("the_emergency_flashing, i ")
+                twpEnd = t.find(")])")
+                tefValue = t[twpBegin+26:twpEnd]
+            if (index+1 < len(trs)) and ("the_indication_lights" not in trs[index+1]) and ("the_flashing_mode" not in trs[index+1]) and ("the_flashing_timer" not in trs[index+1]):
+                item = ["%d" % (time), tvoValue, ttilValue,
+                        tefValue, tilValue, tfmValue, tftValue]
+                table.append(item)
+	    #elif (index+1 == len(trs)):
+		#item = ["%d" % (time), tvoValue, ttilValue,
+                 #       tefValue, tilValue, tfmValue, tftValue]
+                #table.append(item)
+        elif ("the_indication_lights" in t) or ("the_flashing_mode" in t) or ("the_flashing_timer" in t):
+            if "the_indication_lights" in t:
+                tsimBegin = t.find("the_indication_lights, i ")
+                tsimEnd = t.find(")],")
+                tilValue = t[tsimBegin+25:tsimEnd]
+                if len(tilValue) > 5:
+                    tsimEnd = t.find(");")
+                    tilValue = t[tsimBegin+25:tsimEnd]
+            if "the_flashing_mode" in t:
+                tomBegin = t.find("the_flashing_mode, i ")
+                tomEnd = t.find(")],")
+                tfmValue = t[tomBegin+21:tomEnd]
+                if len(tfmValue) > 5:
+                    tomEnd = t.find(");")
+                    tfmValue = t[tomBegin+21:tomEnd]
+            if "the_flashing_timer" in t:
+                tpmBegin = t.find("the_flashing_timer, n ")
+                tpmEnd = t.find(")],")
+                tftValue = t[tpmBegin+22:tpmEnd]
+                if len(tftValue) > 5:
+                    tpmEnd = t.find(");")
+                    tftValue = t[tpmBegin+22:tpmEnd]
+            if (index+1 < len(trs)) and ("the_indication_lights" not in trs[index+1]) and ("the_flashing_mode" not in trs[index+1]) and ("the_flashing_timer" not in trs[index+1]):
+                item = ["%d" % (time), tvoValue, ttilValue,
+                        tefValue, tilValue, tfmValue, tftValue]
+                table.append(item)
+    return table
