run/vmCSV.py
@@ -1,0 +1,58 @@
+#!/usr/bin/env python
+# -*- coding: utf-8 -*-
+
+def generate_table_data(trace):
+    table = [["Time", "I: The_Coin_Sensor", "I: The_Coffee_Request_Button", "O: The_System_Mode", "O: The_Coffee_Machine_Output", "T: The_Request_Timer"],
+            ["0", "false", "false", "1", "0", "0"]]
+    trs = trace.split("[(")
+    time = 0
+    tcsValue = "false"
+    tcrValue = "false"
+    tsmValue = "1"
+    tcmoValue = "0"
+    trtValue = "0"
+    for index, t in enumerate(trs):
+        if "the_coin_sensor" in t:
+            time = time + 1
+            tcsBegin = t.find("the_coin_sensor, b ")
+            tcsEnd = t.find(");")
+            tcsValue = t[tcsBegin+19:tcsEnd]
+            if "the_coffee_request_button" in t:
+                tcrbBegin = t.find("the_coffee_request_button, b ")
+                tcrbEnd = t.find(")])")
+                tcrValue = t[tcrbBegin+29:tcrbEnd]
+            if (index+1 < len(trs)) and ("the_system_mode" not in trs[index+1]) and ("the_request_timer" not in trs[index+1]) and ("the_coffee_machine_output" not in trs[index+1]):
+                item = ["%d" % (time), tcsValue, tcrValue,
+                        tsmValue, tcmoValue, trtValue]
+                table.append(item)
+	    #elif (index+1 == len(trs)):
+		#item = ["%d" % (time), tcsValue, tcrValue,
+                 #       tsmValue, tcmoValue, trtValue]
+                #table.append(item)
+        elif ("the_system_mode" in t) or ("the_request_timer" in t) or ("the_coffee_machine_output" in t):
+            if "the_system_mode" in t:
+                tsmBegin = t.find("the_system_mode, i ")
+                tsmEnd = t.find(")],")
+                tsmValue = t[tsmBegin+19:tsmEnd]
+                if len(tsmValue) > 5:
+                    tsmEnd = t.find(");")
+                    tsmValue = t[tsmBegin+19:tsmEnd]
+            if "the_request_timer" in t:
+                trtBegin = t.find("the_request_timer, n ")
+                trtEnd = t.find(")],")
+                trtValue = t[trtBegin+21:trtEnd]
+                if len(trtValue) > 5:
+                    trtEnd = t.find(");")
+                    trtValue = t[trtBegin+21:trtEnd]
+            if "the_coffee_machine_output" in t:
+                tcmoBegin = t.find("the_coffee_machine_output, i ")
+                tcmoEnd = t.find(")],")
+                tcmoValue = t[tcmoBegin+29:tcmoEnd]
+                if len(tcmoValue) > 5:
+                    tcmoEnd = t.find(");")
+                    tcmoValue = t[tcmoBegin+29:tcmoEnd]
+            if (index+1 < len(trs)) and ("the_system_mode" not in trs[index+1]) and ("the_request_timer" not in trs[index+1]) and ("the_coffee_machine_output" not in trs[index+1]):
+                item = ["%d" % (time), tcsValue, tcrValue,
+                        tsmValue, tcmoValue, trtValue]
+                table.append(item)
+    return table
