src/e_dfrs/e_dfrs_fun_ind_equiv.v
@@ -1,8 +1,166 @@
+Require Import Coq.Lists.List.
+Import ListNotations.
+Require Import Coq.ZArith.ZArith.
+Require Import Bool.
+
+Require Import util_fun_ind_equiv.
 Require Import variables.
+Require Import variables_fun_rules.
+Require Import variables_fun_ind_equiv.
 Require Import states.
+Require Import states_fun_rules.
+Require Import states_fun_ind_equiv.
+Require Import functions.
+Require Import functions_fun_rules.
+Require Import functions_fun_ind_equiv.
 Require Import trans_rel.
+Require Import trans_rel_fun_rules.
+Require Import trans_rel_fun_ind_equiv.
 Require Import e_dfrs.
 Require Import e_dfrs_fun_rules.
+
+Theorem lemm_is_valid_states:
+  forall (states : list STATE) (f : list (NAME * TYPE)),
+    is_valid_states states f <->
+    bis_valid_states states f = true.
+Proof.
+  intros. split.
+  - induction states.
+    + simpl. reflexivity.
+    + simpl. intro. destruct H.
+      rewrite lemm_well_typed_state in H.
+      rewrite H. apply IHstates. apply H0.
+  - induction states.
+    + simpl. reflexivity.
+    + simpl. intro. destruct (bwell_typed_state a f) eqn:H0.
+      * split.
+        { rewrite lemm_well_typed_state. apply H0. }
+        { apply IHstates. apply H. }
+      * split.
+        { inversion H. }
+        { inversion H. }
+Qed.
+
+Theorem lemm_is_valid_trans:
+  forall (trans : list TRANS) (sts : list STATE) 
+  (I O T : list (VNAME * TYPE)) (gcvar : (NAME * TYPE)),
+    is_valid_trans trans sts I O T gcvar <->
+    bis_valid_trans trans sts I O T gcvar = true.
+Proof.
+  intros. split.
+  - induction trans.
+    + simpl. reflexivity.
+    + simpl. intro. destruct H. destruct H0. destruct H1. destruct H2.
+      rewrite lemm_in_list in H.
+      * rewrite lemm_in_list in H0.
+        { rewrite H0. rewrite lemm_well_typed_transition in H1.
+          rewrite H. rewrite H1. simpl. destruct (branFun (snd (fst (STS a)))).
+          - rewrite lemm_eq_state in H2. rewrite H2.
+            destruct (branDel (snd (fst (STS a)))).
+            + destruct (branDiscrete (snd (fst (STS a)))).
+              * destruct (beq_state_elements
+                          (update_gc
+                             (update_state_values (state (fst3 (STS a))) 
+                                (fst3 (STS a)) (map (fun x : VNAME * TYPE => vname (fst x)) T)
+                                (map (fun x : ASGMT => vname (fst (asgmt x)))
+                                   (asgmts
+                                      match delayTransition (snd3 (STS a)) with
+                                      | Some a => snd a
+                                      | None => default_asgmts
+                                      end))
+                                match delayTransition (snd3 (STS a)) with
+                                | Some a => snd a
+                                | None => default_asgmts
+                                end) (state (fst3 (STS a)))
+                             match delayTransition (snd3 (STS a)) with
+                             | Some a => fst a
+                             | None => discrete 0
+                             end) (state (snd (STS a)))).
+                { apply IHtrans in H3. apply H3. }
+                { inversion H3. }
+              * apply IHtrans in H3. apply H3.
+            + apply IHtrans in H3. apply H3.
+          - apply IHtrans in H2. rewrite H2.
+            destruct (branDel (snd (fst (STS a)))).
+            + destruct (branDiscrete (snd (fst (STS a)))).
+              * destruct (beq_state_elements
+                          (update_gc
+                             (update_state_values (state (fst3 (STS a))) 
+                                (fst3 (STS a)) (map (fun x : VNAME * TYPE => vname (fst x)) T)
+                                (map (fun x : ASGMT => vname (fst (asgmt x)))
+                                   (asgmts
+                                      match delayTransition (snd3 (STS a)) with
+                                      | Some a => snd a
+                                      | None => default_asgmts
+                                      end))
+                                match delayTransition (snd3 (STS a)) with
+                                | Some a => snd a
+                                | None => default_asgmts
+                                end) (state (fst3 (STS a)))
+                             match delayTransition (snd3 (STS a)) with
+                             | Some a => fst a
+                             | None => discrete 0
+                             end) (state (snd (STS a)))).
+                { reflexivity. }
+                { inversion H3. }
+              * reflexivity.
+            + reflexivity. }
+        { intros. split.
+          - intro. rewrite lemm_eq_state in H4. apply H4.
+          - intro. rewrite lemm_eq_state. apply H4. }
+      * intros. split.
+        { intro. rewrite lemm_eq_state in H4. apply H4. }
+        { intro. rewrite lemm_eq_state. apply H4. }
+  - induction trans.
+    + simpl. reflexivity.
+    + simpl. intro. 
+      rewrite andb_true_iff in H; destruct H;
+      rewrite andb_true_iff in H; destruct H;
+      rewrite andb_true_iff in H; destruct H;
+      rewrite andb_true_iff in H; destruct H.
+      split.
+      * rewrite lemm_in_list.
+        { apply H. }
+        { intros. split.
+          - intro. rewrite lemm_eq_state in H4. apply H4.
+          - intro. rewrite lemm_eq_state. apply H4. }
+      * split.
+        { rewrite lemm_in_list.
+          - apply H3.
+          - intros. split.
+            + intro. rewrite lemm_eq_state in H4. apply H4.
+            + intro. rewrite lemm_eq_state. apply H4. }
+        { split.
+          - rewrite lemm_well_typed_transition. apply H2.
+          - split.
+            + destruct (branFun (snd (fst (STS a)))).
+              * rewrite lemm_eq_state. apply H1.
+              * apply IHtrans. apply H1.
+            + destruct (branDel (snd (fst (STS a)))).
+              * destruct (branDiscrete (snd (fst (STS a)))).
+                { destruct (beq_state_elements
+                             (update_gc
+                                (update_state_values (state (fst3 (STS a))) 
+                                   (fst3 (STS a)) (map (fun x : VNAME * TYPE => vname (fst x)) T)
+                                   (map (fun x : ASGMT => vname (fst (asgmt x)))
+                                      (asgmts
+                                         match delayTransition (snd3 (STS a)) with
+                                         | Some a0 => snd a0
+                                         | None => default_asgmts
+                                         end))
+                                   match delayTransition (snd3 (STS a)) with
+                                   | Some a0 => snd a0
+                                   | None => default_asgmts
+                                   end) (state (fst3 (STS a)))
+                                match delayTransition (snd3 (STS a)) with
+                                | Some a0 => fst a0
+                                | None => discrete 0
+                                end) (state (snd (STS a)))).
+                  - apply IHtrans. apply H0.
+                  - inversion H0. }
+                { apply IHtrans. apply H0. }
+              * apply IHtrans. apply H0. }
+Qed.
 
 (* E_DFRS *)
 Theorem theo_rules_e_dfrs :
@@ -10,4 +168,12 @@ Theorem theo_rules_e_dfrs :
          (trs : DFRS_TRANSITION_RELATION),
     ind_rules_e_dfrs vars states trs
     <-> fun_rules_e_dfrs vars states trs = true.
-Proof. Admitted.
+Proof. 
+  intros. unfold ind_rules_e_dfrs, fun_rules_e_dfrs. split.
+  - intro. destruct H. rewrite lemm_is_valid_states in H.
+    rewrite lemm_is_valid_trans in H0. rewrite H. rewrite H0.
+    simpl. reflexivity.
+  - intro. rewrite andb_true_iff in H. destruct H. split.
+    + rewrite lemm_is_valid_states. apply H.
+    + rewrite lemm_is_valid_trans. apply H0.
+Qed.
