src/examples/npp/npp_samples.v
@@ -1,0 +1,13 @@
+Require Import npp_tests.
+Require Import qc_instances.
+
+Sample (genValidTrace npp_initial_state npp_s_dfrs npp_possibilities 600).
+Sample (genValidTrace npp_initial_state npp_s_dfrs npp_possibilities 600).
+Sample (genValidTrace npp_initial_state npp_s_dfrs npp_possibilities 600).
+Sample (genValidTrace npp_initial_state npp_s_dfrs npp_possibilities 600).
+Sample (genValidTrace npp_initial_state npp_s_dfrs npp_possibilities 600).
+Sample (genValidTrace npp_initial_state npp_s_dfrs npp_possibilities 600).
+Sample (genValidTrace npp_initial_state npp_s_dfrs npp_possibilities 600).
+Sample (genValidTrace npp_initial_state npp_s_dfrs npp_possibilities 600).
+Sample (genValidTrace npp_initial_state npp_s_dfrs npp_possibilities 600).
+Sample (genValidTrace npp_initial_state npp_s_dfrs npp_possibilities 600).
