src/examples/tis/tis_samples.v
@@ -1,0 +1,13 @@
+Require Import tis_tests.
+Require Import qc_instances.
+
+Sample (genValidTrace tis_initial_state tis_s_dfrs tis_possibilities 600).
+Sample (genValidTrace tis_initial_state tis_s_dfrs tis_possibilities 600).
+Sample (genValidTrace tis_initial_state tis_s_dfrs tis_possibilities 600).
+Sample (genValidTrace tis_initial_state tis_s_dfrs tis_possibilities 600).
+Sample (genValidTrace tis_initial_state tis_s_dfrs tis_possibilities 600).
+Sample (genValidTrace tis_initial_state tis_s_dfrs tis_possibilities 600).
+Sample (genValidTrace tis_initial_state tis_s_dfrs tis_possibilities 600).
+Sample (genValidTrace tis_initial_state tis_s_dfrs tis_possibilities 600).
+Sample (genValidTrace tis_initial_state tis_s_dfrs tis_possibilities 600).
+Sample (genValidTrace tis_initial_state tis_s_dfrs tis_possibilities 600).
