src/s2e_dfrs/properties.v
@@ -1,0 +1,91 @@
+Require Import Coq.Lists.List.
+Import ListNotations.
+
+Require Import states.
+Require Import trans_rel.
+Require Import s_dfrs.
+Require Import e_dfrs.
+Require Import s2e_dfrs_fun_rules.
+
+Fixpoint reached_func_state (sdfrs : s_DFRS) (s : STATE) (trace : list TRANS_LABEL) : STATE :=
+  match trace with
+  | []      => s
+  | h :: tl => let T := sdfrs.(s_dfrs_variables).(T) in
+               match h with
+               | func (a, req) => reached_func_state sdfrs
+                                    (nextState s T.(stimers) a) tl
+               | del _         => s
+               end
+  end.
+  
+Inductive ind_func_trace : s_DFRS -> STATE -> list TRANS_LABEL -> Prop :=
+  | func_traces_empty :
+    forall (sdfrs : s_DFRS) (s : STATE),
+      let I   := sdfrs.(s_dfrs_variables).(I).(svars) in
+      let O   := sdfrs.(s_dfrs_variables).(O).(svars) in
+      let T   := sdfrs.(s_dfrs_variables).(T).(stimers) in
+      let IOT := List.app (List.app I O) T in
+      let All := List.app ([sdfrs.(s_dfrs_variables).(gcvar)])
+                          (map (fun x : (VNAME * TYPE) 
+                            => ((fst x).(vname), snd x)) IOT) in
+      let F := sdfrs.(s_dfrs_functions).(F) in      
+        well_typed_state s All /\
+        (is_stable s (List.app I O) T [F]) = false
+        -> ind_func_trace sdfrs s []
+  | func_traces_step :
+    forall (sdfrs : s_DFRS) (s : STATE) (t : list TRANS_LABEL),
+      let I := sdfrs.(s_dfrs_variables).(I).(svars) in
+      let O := sdfrs.(s_dfrs_variables).(O).(svars) in
+      let T := sdfrs.(s_dfrs_variables).(T).(stimers) in
+      let IOT := List.app (List.app I O) T in
+      let All := List.app ([sdfrs.(s_dfrs_variables).(gcvar)])
+                          (map (fun x : (VNAME * TYPE) 
+                            => ((fst x).(vname), snd x)) IOT) in
+      let F := sdfrs.(s_dfrs_functions).(F) in
+      let entries := union_lists
+                      (map (fun f : FUNCTION => f.(function)) (union_lists [F])) in
+        well_typed_state s All /\
+        (is_stable s (List.app I O) T [F]) = false
+        /\ ind_func_trace sdfrs s t
+        -> forall (s' : STATE), s' = reached_func_state sdfrs s t
+           /\ (is_stable s' (List.app I O) T [F]) = false
+           -> let L := map (fun (t : TRANS) => snd3 t.(STS))
+                           (make_trans_func s' (I ++ O) T entries) in
+              forall (l : TRANS_LABEL), In l L -> ind_func_trace sdfrs s (t ++ [l]).
+
+Definition deterministic (sdfrs: s_DFRS) : Prop :=
+  let I := sdfrs.(s_dfrs_variables).(I).(svars) in
+  let O := sdfrs.(s_dfrs_variables).(O).(svars) in
+  let T := sdfrs.(s_dfrs_variables).(T).(stimers) in
+  let F := sdfrs.(s_dfrs_functions).(F) in
+  forall (s : STATE) (t1 t2 : list TRANS_LABEL),
+    let s1 := reached_func_state sdfrs s t1 in
+    let s2 := reached_func_state sdfrs s t2 in
+    ind_func_trace sdfrs s t1 /\ ind_func_trace sdfrs s t2 /\
+    (is_stable s1 (List.app I O) T [F]) = true /\
+    (is_stable s2 (List.app I O) T [F]) = true
+    -> s1 = s2.
+    
+Fixpoint visited_func_states (sdfrs : s_DFRS) (s : STATE) (trace : list TRANS_LABEL) : list STATE :=
+  match trace with
+  | []      => []
+  | h :: tl => let T := sdfrs.(s_dfrs_variables).(T) in
+               match h with
+               | func (a, req) => s ::
+                                  visited_func_states sdfrs
+                                    (nextState s T.(stimers) a) tl
+               | del _         => []
+               end
+  end.
+
+Fixpoint count_occ_states (l : list STATE) (s : STATE) : nat :=
+  match l with
+  | [] => 0
+  | s' :: tl => let n := count_occ_states tl s in
+                if beq_state s s' then S n else n
+  end.
+
+Definition no_time_lock (sdfrs : s_DFRS) : Prop :=
+  forall (s : STATE) (t : list TRANS_LABEL),
+    let S := visited_func_states sdfrs s t in
+    ind_func_trace sdfrs s t -> count_occ_states S s = 1.
