src/s_dfrs/s_dfrs_fun_ind_equiv.v
@@ -1,14 +1,108 @@
+Require Import util_fun_ind_equiv.
 Require Import variables.
+Require Import variables_fun_rules.
 Require Import states.
+Require Import states_fun_rules.
+Require Import states_fun_ind_equiv.
 Require Import functions.
+Require Import functions_fun_rules.
+Require Import functions_fun_ind_equiv.
 Require Import s_dfrs.
 Require Import s_dfrs_fun_rules.
 
+Require Import Coq.Bool.Bool.
+Require Import Coq.Lists.List.
+Import ListNotations.
+
 (* S_DFRS *)
+
+Theorem lemm_check_function_entries:
+  forall (l : list (EXP * EXP * ASGMTS * REQUIREMENT))
+  (IO T OT : list (VNAME * TYPE)),
+    check_function_entries l IO T OT <->
+    bcheck_function_entries l IO T OT = true.
+Proof.
+  intros. split.
+  - induction l.
+    + simpl. reflexivity.
+    + intro. simpl. simpl in H.
+      destruct H; destruct H0; destruct H1.
+      rewrite andb_true_iff; rewrite andb_true_iff;
+      rewrite andb_true_iff. split.
+      * split.
+        { split.
+          - rewrite lemm_var_consistent_exp in H. apply H.
+          - rewrite lemm_var_consistent_exp in H0. apply H0. }
+        { rewrite lemm_well_typed_asgmts in H1. apply H1. }
+      * apply IHl. apply H2.
+  - induction l.
+    + simpl. reflexivity.
+    + intro. simpl. simpl in H. rewrite andb_true_iff in H
+      ; rewrite andb_true_iff in H; rewrite andb_true_iff in H.
+      destruct H; destruct H; destruct H. split.
+      * rewrite lemm_var_consistent_exp. apply H.
+      * split.
+        { rewrite lemm_var_consistent_exp. apply H2. }
+        { split.
+          - rewrite lemm_well_typed_asgmts. apply H1.
+          - apply IHl. apply H0. }
+Qed.
+
+Theorem lemm_check_functions :
+  forall (lf : list FUNCTION) (IO T OT : list (VNAME * TYPE)),
+    check_functions lf IO T OT <->
+    bcheck_functions lf IO T OT = true.
+Proof.
+  intros. split.
+  - induction lf.
+    + simpl. reflexivity.
+    + intro. simpl. simpl in H. destruct H.
+      rewrite andb_true_iff. split.
+      * rewrite <- lemm_check_function_entries. apply H.
+      * apply IHlf. apply H0.
+  - induction lf.
+    + simpl. reflexivity.
+    + intro. simpl. simpl in H. rewrite andb_true_iff in H.
+      destruct H. split.
+      * rewrite lemm_check_function_entries. apply H.
+      * apply IHlf. apply H0.
+Qed.
 
 Theorem theo_rules_s_dfrs :
   forall (vars : DFRS_VARIABLES) (initial : DFRS_INITIAL_STATE)
          (funs : DFRS_FUNCTIONS),
     ind_rules_s_dfrs vars initial funs
     <-> fun_rules_s_dfrs vars initial funs = true.
-Proof. Admitted.
+Proof. 
+  intros. unfold ind_rules_s_dfrs, fun_rules_s_dfrs. split.
+  - simpl. intros. destruct H.
+    + rewrite lemm_well_typed_state in H. rewrite lemm_check_functions in H0.
+      rewrite H. rewrite H0. simpl. reflexivity.
+  - intros. rewrite lemm_well_typed_state. rewrite lemm_check_functions. split.
+    destruct (bcheck_functions (F funs) (svars (I vars) ++ svars (O vars))
+       (stimers (T vars)) (svars (O vars) ++ stimers (T vars))).
+    + simpl in H. simpl. 
+      destruct (bwell_typed_state (s0 initial)
+       (gcvar vars
+        :: List.map (fun x : VNAME * TYPE => (vname (fst x), snd x))
+             ((svars (I vars) ++ svars (O vars)) ++ stimers (T vars)))).
+      * reflexivity.
+      * inversion H.
+    + simpl in H. simpl.
+      destruct (bwell_typed_state (s0 initial)
+       (gcvar vars
+        :: List.map (fun x : VNAME * TYPE => (vname (fst x), snd x))
+             ((svars (I vars) ++ svars (O vars)) ++ stimers (T vars)))).
+      * reflexivity.
+      * inversion H.
+    + simpl in H.
+      destruct (bwell_typed_state (s0 initial)
+       (gcvar vars
+        :: List.map (fun x : VNAME * TYPE => (vname (fst x), snd x))
+             ((svars (I vars) ++ svars (O vars)) ++ stimers (T vars)))).
+      * destruct (bcheck_functions (F funs) (svars (I vars) ++ svars (O vars))
+       (stimers (T vars)) (svars (O vars) ++ stimers (T vars))).
+        { reflexivity. }
+        { inversion H. }
+      * inversion H.
+Qed.
