analyses/tis_srciror/run.sh
@@ -1,0 +1,1952 @@
+find . -name "output.txt" -exec rm -rf {} \;
+date +%s ;gcc main1.c -o main1;
+gcc main2.c -o main2;
+gcc main3.c -o main3;
+gcc main4.c -o main4;
+gcc main5.c -o main5;
+gcc main6.c -o main6;
+gcc main7.c -o main7;
+gcc main8.c -o main8;
+gcc main9.c -o main9;
+gcc main10.c -o main10;
+gcc main11.c -o main11;
+gcc main12.c -o main12;
+gcc main13.c -o main13;
+gcc main14.c -o main14;
+gcc main15.c -o main15;
+gcc main16.c -o main16;
+gcc main17.c -o main17;
+gcc main18.c -o main18;
+gcc main19.c -o main19;
+gcc main20.c -o main20;
+gcc main21.c -o main21;
+gcc main22.c -o main22;
+gcc main23.c -o main23;
+gcc main24.c -o main24;
+gcc main25.c -o main25;
+gcc main26.c -o main26;
+gcc main27.c -o main27;
+gcc main28.c -o main28;
+gcc main29.c -o main29;
+gcc main30.c -o main30;
+gcc main31.c -o main31;
+gcc main32.c -o main32;
+gcc main33.c -o main33;
+gcc main34.c -o main34;
+gcc main35.c -o main35;
+gcc main36.c -o main36;
+gcc main37.c -o main37;
+gcc main38.c -o main38;
+gcc main39.c -o main39;
+gcc main40.c -o main40;
+gcc main41.c -o main41;
+gcc main42.c -o main42;
+gcc main43.c -o main43;
+gcc main44.c -o main44;
+gcc main45.c -o main45;
+gcc main46.c -o main46;
+gcc main47.c -o main47;
+gcc main48.c -o main48;
+gcc main49.c -o main49;
+gcc main50.c -o main50;
+gcc main51.c -o main51;
+gcc main52.c -o main52;
+gcc main53.c -o main53;
+gcc main54.c -o main54;
+gcc main55.c -o main55;
+gcc main56.c -o main56;
+gcc main57.c -o main57;
+gcc main58.c -o main58;
+gcc main59.c -o main59;
+gcc main60.c -o main60;
+gcc main61.c -o main61;
+gcc main62.c -o main62;
+gcc main63.c -o main63;
+gcc main64.c -o main64;
+gcc main65.c -o main65;
+gcc main66.c -o main66;
+gcc main67.c -o main67;
+gcc main68.c -o main68;
+gcc main69.c -o main69;
+gcc main70.c -o main70;
+gcc main71.c -o main71;
+gcc main72.c -o main72;
+gcc main73.c -o main73;
+gcc main74.c -o main74;
+gcc main75.c -o main75;
+gcc main76.c -o main76;
+gcc main77.c -o main77;
+gcc main78.c -o main78;
+gcc main79.c -o main79;
+gcc main80.c -o main80;
+gcc main81.c -o main81;
+gcc main82.c -o main82;
+gcc main83.c -o main83;
+gcc main84.c -o main84;
+gcc main85.c -o main85;
+gcc main86.c -o main86;
+gcc main87.c -o main87;
+gcc main88.c -o main88;
+gcc main89.c -o main89;
+gcc main90.c -o main90;
+gcc main91.c -o main91;
+gcc main92.c -o main92;
+gcc main93.c -o main93;
+gcc main94.c -o main94;
+gcc main95.c -o main95;
+gcc main96.c -o main96;
+gcc main97.c -o main97;
+gcc main98.c -o main98;
+gcc main99.c -o main99;
+gcc main100.c -o main100;
+gcc main101.c -o main101;
+gcc main102.c -o main102;
+gcc main103.c -o main103;
+gcc main104.c -o main104;
+gcc main105.c -o main105;
+gcc main106.c -o main106;
+gcc main107.c -o main107;
+gcc main108.c -o main108;
+gcc main109.c -o main109;
+gcc main110.c -o main110;
+gcc main111.c -o main111;
+gcc main112.c -o main112;
+gcc main113.c -o main113;
+gcc main114.c -o main114;
+gcc main115.c -o main115;
+gcc main116.c -o main116;
+gcc main117.c -o main117;
+gcc main118.c -o main118;
+gcc main119.c -o main119;
+gcc main120.c -o main120;
+gcc main121.c -o main121;
+gcc main122.c -o main122;
+gcc main123.c -o main123;
+gcc main124.c -o main124;
+gcc main125.c -o main125;
+gcc main126.c -o main126;
+gcc main127.c -o main127;
+gcc main128.c -o main128;
+gcc main129.c -o main129;
+gcc main130.c -o main130;
+gcc main131.c -o main131;
+gcc main132.c -o main132;
+gcc main133.c -o main133;
+gcc main134.c -o main134;
+gcc main135.c -o main135;
+gcc main136.c -o main136;
+gcc main137.c -o main137;
+gcc main138.c -o main138;
+gcc main139.c -o main139;
+gcc main140.c -o main140;
+gcc main141.c -o main141;
+gcc main142.c -o main142;
+gcc main143.c -o main143;
+gcc main144.c -o main144;
+gcc main145.c -o main145;
+gcc main146.c -o main146;
+gcc main147.c -o main147;
+gcc main148.c -o main148;
+gcc main149.c -o main149;
+gcc main150.c -o main150;
+gcc main151.c -o main151;
+gcc main152.c -o main152;
+gcc main153.c -o main153;
+gcc main154.c -o main154;
+gcc main155.c -o main155;
+gcc main156.c -o main156;
+gcc main157.c -o main157;
+gcc main158.c -o main158;
+gcc main159.c -o main159;
+gcc main160.c -o main160;
+gcc main161.c -o main161;
+gcc main162.c -o main162;
+gcc main163.c -o main163;
+gcc main164.c -o main164;
+gcc main165.c -o main165;
+gcc main166.c -o main166;
+gcc main167.c -o main167;
+gcc main168.c -o main168;
+gcc main169.c -o main169;
+gcc main170.c -o main170;
+gcc main171.c -o main171;
+gcc main172.c -o main172;
+gcc main173.c -o main173;
+gcc main174.c -o main174;
+gcc main175.c -o main175;
+gcc main176.c -o main176;
+gcc main177.c -o main177;
+gcc main178.c -o main178;
+gcc main179.c -o main179;
+gcc main180.c -o main180;
+gcc main181.c -o main181;
+gcc main182.c -o main182;
+gcc main183.c -o main183;
+gcc main184.c -o main184;
+gcc main185.c -o main185;
+gcc main186.c -o main186;
+gcc main187.c -o main187;
+gcc main188.c -o main188;
+gcc main189.c -o main189;
+gcc main190.c -o main190;
+gcc main191.c -o main191;
+gcc main192.c -o main192;
+gcc main193.c -o main193;
+gcc main194.c -o main194;
+gcc main195.c -o main195;
+gcc main196.c -o main196;
+gcc main197.c -o main197;
+gcc main198.c -o main198;
+gcc main199.c -o main199;
+gcc main200.c -o main200;
+gcc main201.c -o main201;
+gcc main202.c -o main202;
+gcc main203.c -o main203;
+gcc main204.c -o main204;
+gcc main205.c -o main205;
+gcc main206.c -o main206;
+gcc main207.c -o main207;
+gcc main208.c -o main208;
+gcc main209.c -o main209;
+gcc main210.c -o main210;
+gcc main211.c -o main211;
+gcc main212.c -o main212;
+gcc main213.c -o main213;
+gcc main214.c -o main214;
+gcc main215.c -o main215;
+gcc main216.c -o main216;
+gcc main217.c -o main217;
+gcc main218.c -o main218;
+gcc main219.c -o main219;
+gcc main220.c -o main220;
+gcc main221.c -o main221;
+gcc main222.c -o main222;
+gcc main223.c -o main223;
+gcc main224.c -o main224;
+gcc main225.c -o main225;
+gcc main226.c -o main226;
+gcc main227.c -o main227;
+gcc main228.c -o main228;
+gcc main229.c -o main229;
+gcc main230.c -o main230;
+gcc main231.c -o main231;
+gcc main232.c -o main232;
+gcc main233.c -o main233;
+gcc main234.c -o main234;
+gcc main235.c -o main235;
+gcc main236.c -o main236;
+gcc main237.c -o main237;
+gcc main238.c -o main238;
+gcc main239.c -o main239;
+gcc main240.c -o main240;
+gcc main241.c -o main241;
+gcc main242.c -o main242;
+gcc main243.c -o main243;
+gcc main244.c -o main244;
+gcc main245.c -o main245;
+gcc main246.c -o main246;
+gcc main247.c -o main247;
+gcc main248.c -o main248;
+gcc main249.c -o main249;
+gcc main250.c -o main250;
+gcc main251.c -o main251;
+gcc main252.c -o main252;
+gcc main253.c -o main253;
+gcc main254.c -o main254;
+gcc main255.c -o main255;
+gcc main256.c -o main256;
+gcc main257.c -o main257;
+gcc main258.c -o main258;
+gcc main259.c -o main259;
+gcc main260.c -o main260;
+gcc main261.c -o main261;
+gcc main262.c -o main262;
+gcc main263.c -o main263;
+gcc main264.c -o main264;
+gcc main265.c -o main265;
+gcc main266.c -o main266;
+gcc main267.c -o main267;
+gcc main268.c -o main268;
+gcc main269.c -o main269;
+gcc main270.c -o main270;
+gcc main271.c -o main271;
+gcc main272.c -o main272;
+gcc main273.c -o main273;
+gcc main274.c -o main274;
+gcc main275.c -o main275;
+gcc main276.c -o main276;
+gcc main277.c -o main277;
+gcc main278.c -o main278;
+gcc main279.c -o main279;
+gcc main280.c -o main280;
+gcc main281.c -o main281;
+gcc main282.c -o main282;
+gcc main283.c -o main283;
+gcc main284.c -o main284;
+gcc main285.c -o main285;
+gcc main286.c -o main286;
+gcc main287.c -o main287;
+gcc main288.c -o main288;
+gcc main289.c -o main289;
+gcc main290.c -o main290;
+gcc main291.c -o main291;
+gcc main292.c -o main292;
+gcc main293.c -o main293;
+gcc main294.c -o main294;
+gcc main295.c -o main295;
+gcc main296.c -o main296;
+gcc main297.c -o main297;
+gcc main298.c -o main298;
+gcc main299.c -o main299;
+gcc main300.c -o main300;
+gcc main301.c -o main301;
+gcc main302.c -o main302;
+gcc main303.c -o main303;
+gcc main304.c -o main304;
+gcc main305.c -o main305;
+gcc main306.c -o main306;
+gcc main307.c -o main307;
+gcc main308.c -o main308;
+gcc main309.c -o main309;
+gcc main310.c -o main310;
+gcc main311.c -o main311;
+gcc main312.c -o main312;
+gcc main313.c -o main313;
+gcc main314.c -o main314;
+gcc main315.c -o main315;
+gcc main316.c -o main316;
+gcc main317.c -o main317;
+gcc main318.c -o main318;
+gcc main319.c -o main319;
+gcc main320.c -o main320;
+gcc main321.c -o main321;
+gcc main322.c -o main322;
+gcc main323.c -o main323;
+gcc main324.c -o main324;
+gcc main325.c -o main325;
+gcc main326.c -o main326;
+gcc main327.c -o main327;
+gcc main328.c -o main328;
+gcc main329.c -o main329;
+gcc main330.c -o main330;
+gcc main331.c -o main331;
+gcc main332.c -o main332;
+gcc main333.c -o main333;
+gcc main334.c -o main334;
+gcc main335.c -o main335;
+gcc main336.c -o main336;
+gcc main337.c -o main337;
+gcc main338.c -o main338;
+gcc main339.c -o main339;
+gcc main340.c -o main340;
+gcc main341.c -o main341;
+gcc main342.c -o main342;
+gcc main343.c -o main343;
+gcc main344.c -o main344;
+gcc main345.c -o main345;
+gcc main346.c -o main346;
+gcc main347.c -o main347;
+gcc main348.c -o main348;
+gcc main349.c -o main349;
+gcc main350.c -o main350;
+gcc main351.c -o main351;
+gcc main352.c -o main352;
+gcc main353.c -o main353;
+gcc main354.c -o main354;
+gcc main355.c -o main355;
+gcc main356.c -o main356;
+gcc main357.c -o main357;
+gcc main358.c -o main358;
+gcc main359.c -o main359;
+gcc main360.c -o main360;
+gcc main361.c -o main361;
+gcc main362.c -o main362;
+gcc main363.c -o main363;
+gcc main364.c -o main364;
+gcc main365.c -o main365;
+gcc main366.c -o main366;
+gcc main367.c -o main367;
+gcc main368.c -o main368;
+gcc main369.c -o main369;
+gcc main370.c -o main370;
+gcc main371.c -o main371;
+gcc main372.c -o main372;
+gcc main373.c -o main373;
+gcc main374.c -o main374;
+gcc main375.c -o main375;
+gcc main376.c -o main376;
+gcc main377.c -o main377;
+gcc main378.c -o main378;
+gcc main379.c -o main379;
+gcc main380.c -o main380;
+gcc main381.c -o main381;
+gcc main382.c -o main382;
+gcc main383.c -o main383;
+gcc main384.c -o main384;
+gcc main385.c -o main385;
+gcc main386.c -o main386;
+gcc main387.c -o main387;
+gcc main388.c -o main388;
+gcc main389.c -o main389;
+gcc main390.c -o main390;
+gcc main391.c -o main391;
+gcc main392.c -o main392;
+gcc main393.c -o main393;
+gcc main394.c -o main394;
+gcc main395.c -o main395;
+gcc main396.c -o main396;
+gcc main397.c -o main397;
+gcc main398.c -o main398;
+gcc main399.c -o main399;
+gcc main400.c -o main400;
+gcc main401.c -o main401;
+gcc main402.c -o main402;
+gcc main403.c -o main403;
+gcc main404.c -o main404;
+gcc main405.c -o main405;
+gcc main406.c -o main406;
+gcc main407.c -o main407;
+gcc main408.c -o main408;
+gcc main409.c -o main409;
+gcc main410.c -o main410;
+gcc main411.c -o main411;
+gcc main412.c -o main412;
+gcc main413.c -o main413;
+gcc main414.c -o main414;
+gcc main415.c -o main415;
+gcc main416.c -o main416;
+gcc main417.c -o main417;
+gcc main418.c -o main418;
+gcc main419.c -o main419;
+gcc main420.c -o main420;
+gcc main421.c -o main421;
+gcc main422.c -o main422;
+gcc main423.c -o main423;
+gcc main424.c -o main424;
+gcc main425.c -o main425;
+gcc main426.c -o main426;
+gcc main427.c -o main427;
+gcc main428.c -o main428;
+gcc main429.c -o main429;
+gcc main430.c -o main430;
+gcc main431.c -o main431;
+gcc main432.c -o main432;
+gcc main433.c -o main433;
+gcc main434.c -o main434;
+gcc main435.c -o main435;
+gcc main436.c -o main436;
+gcc main437.c -o main437;
+gcc main438.c -o main438;
+gcc main439.c -o main439;
+gcc main440.c -o main440;
+gcc main441.c -o main441;
+gcc main442.c -o main442;
+gcc main443.c -o main443;
+gcc main444.c -o main444;
+gcc main445.c -o main445;
+gcc main446.c -o main446;
+gcc main447.c -o main447;
+gcc main448.c -o main448;
+gcc main449.c -o main449;
+gcc main450.c -o main450;
+gcc main451.c -o main451;
+gcc main452.c -o main452;
+gcc main453.c -o main453;
+gcc main454.c -o main454;
+gcc main455.c -o main455;
+gcc main456.c -o main456;
+gcc main457.c -o main457;
+gcc main458.c -o main458;
+gcc main459.c -o main459;
+gcc main460.c -o main460;
+gcc main461.c -o main461;
+gcc main462.c -o main462;
+gcc main463.c -o main463;
+gcc main464.c -o main464;
+gcc main465.c -o main465;
+gcc main466.c -o main466;
+gcc main467.c -o main467;
+gcc main468.c -o main468;
+gcc main469.c -o main469;
+gcc main470.c -o main470;
+gcc main471.c -o main471;
+gcc main472.c -o main472;
+gcc main473.c -o main473;
+gcc main474.c -o main474;
+gcc main475.c -o main475;
+gcc main476.c -o main476;
+gcc main477.c -o main477;
+gcc main478.c -o main478;
+gcc main479.c -o main479;
+gcc main480.c -o main480;
+gcc main481.c -o main481;
+gcc main482.c -o main482;
+gcc main483.c -o main483;
+gcc main484.c -o main484;
+gcc main485.c -o main485;
+gcc main486.c -o main486;
+gcc main487.c -o main487;
+gcc main488.c -o main488;
+gcc main489.c -o main489;
+gcc main490.c -o main490;
+gcc main491.c -o main491;
+gcc main492.c -o main492;
+gcc main493.c -o main493;
+gcc main494.c -o main494;
+gcc main495.c -o main495;
+gcc main496.c -o main496;
+gcc main497.c -o main497;
+gcc main498.c -o main498;
+gcc main499.c -o main499;
+gcc main500.c -o main500;
+gcc main501.c -o main501;
+gcc main502.c -o main502;
+gcc main503.c -o main503;
+gcc main504.c -o main504;
+gcc main505.c -o main505;
+gcc main506.c -o main506;
+gcc main507.c -o main507;
+gcc main508.c -o main508;
+gcc main509.c -o main509;
+gcc main510.c -o main510;
+gcc main511.c -o main511;
+gcc main512.c -o main512;
+gcc main513.c -o main513;
+gcc main514.c -o main514;
+gcc main515.c -o main515;
+gcc main516.c -o main516;
+gcc main517.c -o main517;
+gcc main518.c -o main518;
+gcc main519.c -o main519;
+gcc main520.c -o main520;
+gcc main521.c -o main521;
+gcc main522.c -o main522;
+gcc main523.c -o main523;
+gcc main524.c -o main524;
+gcc main525.c -o main525;
+gcc main526.c -o main526;
+gcc main527.c -o main527;
+gcc main528.c -o main528;
+gcc main529.c -o main529;
+gcc main530.c -o main530;
+gcc main531.c -o main531;
+gcc main532.c -o main532;
+gcc main533.c -o main533;
+gcc main534.c -o main534;
+gcc main535.c -o main535;
+gcc main536.c -o main536;
+gcc main537.c -o main537;
+gcc main538.c -o main538;
+gcc main539.c -o main539;
+gcc main540.c -o main540;
+gcc main541.c -o main541;
+gcc main542.c -o main542;
+gcc main543.c -o main543;
+gcc main544.c -o main544;
+gcc main545.c -o main545;
+gcc main546.c -o main546;
+gcc main547.c -o main547;
+gcc main548.c -o main548;
+gcc main549.c -o main549;
+gcc main550.c -o main550;
+gcc main551.c -o main551;
+gcc main552.c -o main552;
+gcc main553.c -o main553;
+gcc main554.c -o main554;
+gcc main555.c -o main555;
+gcc main556.c -o main556;
+gcc main557.c -o main557;
+gcc main558.c -o main558;
+gcc main559.c -o main559;
+gcc main560.c -o main560;
+gcc main561.c -o main561;
+gcc main562.c -o main562;
+gcc main563.c -o main563;
+gcc main564.c -o main564;
+gcc main565.c -o main565;
+gcc main566.c -o main566;
+gcc main567.c -o main567;
+gcc main568.c -o main568;
+gcc main569.c -o main569;
+gcc main570.c -o main570;
+gcc main571.c -o main571;
+gcc main572.c -o main572;
+gcc main573.c -o main573;
+gcc main574.c -o main574;
+gcc main575.c -o main575;
+gcc main576.c -o main576;
+gcc main577.c -o main577;
+gcc main578.c -o main578;
+gcc main579.c -o main579;
+gcc main580.c -o main580;
+gcc main581.c -o main581;
+gcc main582.c -o main582;
+gcc main583.c -o main583;
+gcc main584.c -o main584;
+gcc main585.c -o main585;
+gcc main586.c -o main586;
+gcc main587.c -o main587;
+gcc main588.c -o main588;
+gcc main589.c -o main589;
+gcc main590.c -o main590;
+gcc main591.c -o main591;
+gcc main592.c -o main592;
+gcc main593.c -o main593;
+gcc main594.c -o main594;
+gcc main595.c -o main595;
+gcc main596.c -o main596;
+gcc main597.c -o main597;
+gcc main598.c -o main598;
+gcc main599.c -o main599;
+gcc main600.c -o main600;
+gcc main601.c -o main601;
+gcc main602.c -o main602;
+gcc main603.c -o main603;
+gcc main604.c -o main604;
+gcc main605.c -o main605;
+gcc main606.c -o main606;
+gcc main607.c -o main607;
+gcc main608.c -o main608;
+gcc main609.c -o main609;
+gcc main610.c -o main610;
+gcc main611.c -o main611;
+gcc main612.c -o main612;
+gcc main613.c -o main613;
+gcc main614.c -o main614;
+gcc main615.c -o main615;
+gcc main616.c -o main616;
+gcc main617.c -o main617;
+gcc main618.c -o main618;
+gcc main619.c -o main619;
+gcc main620.c -o main620;
+gcc main621.c -o main621;
+gcc main622.c -o main622;
+gcc main623.c -o main623;
+gcc main624.c -o main624;
+gcc main625.c -o main625;
+gcc main626.c -o main626;
+gcc main627.c -o main627;
+gcc main628.c -o main628;
+gcc main629.c -o main629;
+gcc main630.c -o main630;
+gcc main631.c -o main631;
+gcc main632.c -o main632;
+gcc main633.c -o main633;
+gcc main634.c -o main634;
+gcc main635.c -o main635;
+gcc main636.c -o main636;
+gcc main637.c -o main637;
+gcc main638.c -o main638;
+gcc main639.c -o main639;
+gcc main640.c -o main640;
+gcc main641.c -o main641;
+gcc main642.c -o main642;
+gcc main643.c -o main643;
+gcc main644.c -o main644;
+gcc main645.c -o main645;
+gcc main646.c -o main646;
+gcc main647.c -o main647;
+gcc main648.c -o main648;
+gcc main649.c -o main649;
+gcc main650.c -o main650;
+gcc main651.c -o main651;
+gcc main652.c -o main652;
+gcc main653.c -o main653;
+gcc main654.c -o main654;
+gcc main655.c -o main655;
+gcc main656.c -o main656;
+gcc main657.c -o main657;
+gcc main658.c -o main658;
+gcc main659.c -o main659;
+gcc main660.c -o main660;
+gcc main661.c -o main661;
+gcc main662.c -o main662;
+gcc main663.c -o main663;
+gcc main664.c -o main664;
+gcc main665.c -o main665;
+gcc main666.c -o main666;
+gcc main667.c -o main667;
+gcc main668.c -o main668;
+gcc main669.c -o main669;
+gcc main670.c -o main670;
+gcc main671.c -o main671;
+gcc main672.c -o main672;
+gcc main673.c -o main673;
+gcc main674.c -o main674;
+gcc main675.c -o main675;
+gcc main676.c -o main676;
+gcc main677.c -o main677;
+gcc main678.c -o main678;
+gcc main679.c -o main679;
+gcc main680.c -o main680;
+gcc main681.c -o main681;
+gcc main682.c -o main682;
+gcc main683.c -o main683;
+gcc main684.c -o main684;
+gcc main685.c -o main685;
+gcc main686.c -o main686;
+gcc main687.c -o main687;
+gcc main688.c -o main688;
+gcc main689.c -o main689;
+gcc main690.c -o main690;
+gcc main691.c -o main691;
+gcc main692.c -o main692;
+gcc main693.c -o main693;
+gcc main694.c -o main694;
+gcc main695.c -o main695;
+gcc main696.c -o main696;
+gcc main697.c -o main697;
+gcc main698.c -o main698;
+gcc main699.c -o main699;
+gcc main700.c -o main700;
+gcc main701.c -o main701;
+gcc main702.c -o main702;
+gcc main703.c -o main703;
+gcc main704.c -o main704;
+gcc main705.c -o main705;
+gcc main706.c -o main706;
+gcc main707.c -o main707;
+gcc main708.c -o main708;
+gcc main709.c -o main709;
+gcc main710.c -o main710;
+gcc main711.c -o main711;
+gcc main712.c -o main712;
+gcc main713.c -o main713;
+gcc main714.c -o main714;
+gcc main715.c -o main715;
+gcc main716.c -o main716;
+gcc main717.c -o main717;
+gcc main718.c -o main718;
+gcc main719.c -o main719;
+gcc main720.c -o main720;
+gcc main721.c -o main721;
+gcc main722.c -o main722;
+gcc main723.c -o main723;
+gcc main724.c -o main724;
+gcc main725.c -o main725;
+gcc main726.c -o main726;
+gcc main727.c -o main727;
+gcc main728.c -o main728;
+gcc main729.c -o main729;
+gcc main730.c -o main730;
+gcc main731.c -o main731;
+gcc main732.c -o main732;
+gcc main733.c -o main733;
+gcc main734.c -o main734;
+gcc main735.c -o main735;
+gcc main736.c -o main736;
+gcc main737.c -o main737;
+gcc main738.c -o main738;
+gcc main739.c -o main739;
+gcc main740.c -o main740;
+gcc main741.c -o main741;
+gcc main742.c -o main742;
+gcc main743.c -o main743;
+gcc main744.c -o main744;
+gcc main745.c -o main745;
+gcc main746.c -o main746;
+gcc main747.c -o main747;
+gcc main748.c -o main748;
+gcc main749.c -o main749;
+gcc main750.c -o main750;
+gcc main751.c -o main751;
+gcc main752.c -o main752;
+gcc main753.c -o main753;
+gcc main754.c -o main754;
+gcc main755.c -o main755;
+gcc main756.c -o main756;
+gcc main757.c -o main757;
+gcc main758.c -o main758;
+gcc main759.c -o main759;
+gcc main760.c -o main760;
+gcc main761.c -o main761;
+gcc main762.c -o main762;
+gcc main763.c -o main763;
+gcc main764.c -o main764;
+gcc main765.c -o main765;
+gcc main766.c -o main766;
+gcc main767.c -o main767;
+gcc main768.c -o main768;
+gcc main769.c -o main769;
+gcc main770.c -o main770;
+gcc main771.c -o main771;
+gcc main772.c -o main772;
+gcc main773.c -o main773;
+gcc main774.c -o main774;
+gcc main775.c -o main775;
+gcc main776.c -o main776;
+gcc main777.c -o main777;
+gcc main778.c -o main778;
+gcc main779.c -o main779;
+gcc main780.c -o main780;
+gcc main781.c -o main781;
+gcc main782.c -o main782;
+gcc main783.c -o main783;
+gcc main784.c -o main784;
+gcc main785.c -o main785;
+gcc main786.c -o main786;
+gcc main787.c -o main787;
+gcc main788.c -o main788;
+gcc main789.c -o main789;
+gcc main790.c -o main790;
+gcc main791.c -o main791;
+gcc main792.c -o main792;
+gcc main793.c -o main793;
+gcc main794.c -o main794;
+gcc main795.c -o main795;
+gcc main796.c -o main796;
+gcc main797.c -o main797;
+gcc main798.c -o main798;
+gcc main799.c -o main799;
+gcc main800.c -o main800;
+gcc main801.c -o main801;
+gcc main802.c -o main802;
+gcc main803.c -o main803;
+gcc main804.c -o main804;
+gcc main805.c -o main805;
+gcc main806.c -o main806;
+gcc main807.c -o main807;
+gcc main808.c -o main808;
+gcc main809.c -o main809;
+gcc main810.c -o main810;
+gcc main811.c -o main811;
+gcc main812.c -o main812;
+gcc main813.c -o main813;
+gcc main814.c -o main814;
+gcc main815.c -o main815;
+gcc main816.c -o main816;
+gcc main817.c -o main817;
+gcc main818.c -o main818;
+gcc main819.c -o main819;
+gcc main820.c -o main820;
+gcc main821.c -o main821;
+gcc main822.c -o main822;
+gcc main823.c -o main823;
+gcc main824.c -o main824;
+gcc main825.c -o main825;
+gcc main826.c -o main826;
+gcc main827.c -o main827;
+gcc main828.c -o main828;
+gcc main829.c -o main829;
+gcc main830.c -o main830;
+gcc main831.c -o main831;
+gcc main832.c -o main832;
+gcc main833.c -o main833;
+gcc main834.c -o main834;
+gcc main835.c -o main835;
+gcc main836.c -o main836;
+gcc main837.c -o main837;
+gcc main838.c -o main838;
+gcc main839.c -o main839;
+gcc main840.c -o main840;
+gcc main841.c -o main841;
+gcc main842.c -o main842;
+gcc main843.c -o main843;
+gcc main844.c -o main844;
+gcc main845.c -o main845;
+gcc main846.c -o main846;
+gcc main847.c -o main847;
+gcc main848.c -o main848;
+gcc main849.c -o main849;
+gcc main850.c -o main850;
+gcc main851.c -o main851;
+gcc main852.c -o main852;
+gcc main853.c -o main853;
+gcc main854.c -o main854;
+gcc main855.c -o main855;
+gcc main856.c -o main856;
+gcc main857.c -o main857;
+gcc main858.c -o main858;
+gcc main859.c -o main859;
+gcc main860.c -o main860;
+gcc main861.c -o main861;
+gcc main862.c -o main862;
+gcc main863.c -o main863;
+gcc main864.c -o main864;
+gcc main865.c -o main865;
+gcc main866.c -o main866;
+gcc main867.c -o main867;
+gcc main868.c -o main868;
+gcc main869.c -o main869;
+gcc main870.c -o main870;
+gcc main871.c -o main871;
+gcc main872.c -o main872;
+gcc main873.c -o main873;
+gcc main874.c -o main874;
+gcc main875.c -o main875;
+gcc main876.c -o main876;
+gcc main877.c -o main877;
+gcc main878.c -o main878;
+gcc main879.c -o main879;
+gcc main880.c -o main880;
+gcc main881.c -o main881;
+gcc main882.c -o main882;
+gcc main883.c -o main883;
+gcc main884.c -o main884;
+gcc main885.c -o main885;
+gcc main886.c -o main886;
+gcc main887.c -o main887;
+gcc main888.c -o main888;
+gcc main889.c -o main889;
+gcc main890.c -o main890;
+gcc main891.c -o main891;
+gcc main892.c -o main892;
+gcc main893.c -o main893;
+gcc main894.c -o main894;
+gcc main895.c -o main895;
+gcc main896.c -o main896;
+gcc main897.c -o main897;
+gcc main898.c -o main898;
+gcc main899.c -o main899;
+gcc main900.c -o main900;
+gcc main901.c -o main901;
+gcc main902.c -o main902;
+gcc main903.c -o main903;
+gcc main904.c -o main904;
+gcc main905.c -o main905;
+gcc main906.c -o main906;
+gcc main907.c -o main907;
+gcc main908.c -o main908;
+gcc main909.c -o main909;
+gcc main910.c -o main910;
+gcc main911.c -o main911;
+gcc main912.c -o main912;
+gcc main913.c -o main913;
+gcc main914.c -o main914;
+gcc main915.c -o main915;
+gcc main916.c -o main916;
+gcc main917.c -o main917;
+gcc main918.c -o main918;
+gcc main919.c -o main919;
+gcc main920.c -o main920;
+gcc main921.c -o main921;
+gcc main922.c -o main922;
+gcc main923.c -o main923;
+gcc main924.c -o main924;
+gcc main925.c -o main925;
+gcc main926.c -o main926;
+gcc main927.c -o main927;
+gcc main928.c -o main928;
+gcc main929.c -o main929;
+gcc main930.c -o main930;
+gcc main931.c -o main931;
+gcc main932.c -o main932;
+gcc main933.c -o main933;
+gcc main934.c -o main934;
+gcc main935.c -o main935;
+gcc main936.c -o main936;
+gcc main937.c -o main937;
+gcc main938.c -o main938;
+gcc main939.c -o main939;
+gcc main940.c -o main940;
+gcc main941.c -o main941;
+gcc main942.c -o main942;
+gcc main943.c -o main943;
+gcc main944.c -o main944;
+gcc main945.c -o main945;
+gcc main946.c -o main946;
+gcc main947.c -o main947;
+gcc main948.c -o main948;
+gcc main949.c -o main949;
+gcc main950.c -o main950;
+gcc main951.c -o main951;
+gcc main952.c -o main952;
+gcc main953.c -o main953;
+gcc main954.c -o main954;
+gcc main955.c -o main955;
+gcc main956.c -o main956;
+gcc main957.c -o main957;
+gcc main958.c -o main958;
+gcc main959.c -o main959;
+gcc main960.c -o main960;
+gcc main961.c -o main961;
+gcc main962.c -o main962;
+gcc main963.c -o main963;
+gcc main964.c -o main964;
+gcc main965.c -o main965;
+gcc main966.c -o main966;
+gcc main967.c -o main967;
+gcc main968.c -o main968;
+gcc main969.c -o main969;
+gcc main970.c -o main970;
+gcc main971.c -o main971;
+gcc main972.c -o main972;
+gcc main973.c -o main973;
+gcc main974.c -o main974;
+gcc main975.c -o main975;
+./main1 >> output.txt
+./main2 >> output.txt
+./main3 >> output.txt
+./main4 >> output.txt
+./main5 >> output.txt
+./main6 >> output.txt
+./main7 >> output.txt
+./main8 >> output.txt
+./main9 >> output.txt
+./main10 >> output.txt
+./main11 >> output.txt
+./main12 >> output.txt
+./main13 >> output.txt
+./main14 >> output.txt
+./main15 >> output.txt
+./main16 >> output.txt
+./main17 >> output.txt
+./main18 >> output.txt
+./main19 >> output.txt
+./main20 >> output.txt
+./main21 >> output.txt
+./main22 >> output.txt
+./main23 >> output.txt
+./main24 >> output.txt
+./main25 >> output.txt
+./main26 >> output.txt
+./main27 >> output.txt
+./main28 >> output.txt
+./main29 >> output.txt
+./main30 >> output.txt
+./main31 >> output.txt
+./main32 >> output.txt
+./main33 >> output.txt
+./main34 >> output.txt
+./main35 >> output.txt
+./main36 >> output.txt
+./main37 >> output.txt
+./main38 >> output.txt
+./main39 >> output.txt
+./main40 >> output.txt
+./main41 >> output.txt
+./main42 >> output.txt
+./main43 >> output.txt
+./main44 >> output.txt
+./main45 >> output.txt
+./main46 >> output.txt
+./main47 >> output.txt
+./main48 >> output.txt
+./main49 >> output.txt
+./main50 >> output.txt
+./main51 >> output.txt
+./main52 >> output.txt
+./main53 >> output.txt
+./main54 >> output.txt
+./main55 >> output.txt
+./main56 >> output.txt
+./main57 >> output.txt
+./main58 >> output.txt
+./main59 >> output.txt
+./main60 >> output.txt
+./main61 >> output.txt
+./main62 >> output.txt
+./main63 >> output.txt
+./main64 >> output.txt
+./main65 >> output.txt
+./main66 >> output.txt
+./main67 >> output.txt
+./main68 >> output.txt
+./main69 >> output.txt
+./main70 >> output.txt
+./main71 >> output.txt
+./main72 >> output.txt
+./main73 >> output.txt
+./main74 >> output.txt
+./main75 >> output.txt
+./main76 >> output.txt
+./main77 >> output.txt
+./main78 >> output.txt
+./main79 >> output.txt
+./main80 >> output.txt
+./main81 >> output.txt
+./main82 >> output.txt
+./main83 >> output.txt
+./main84 >> output.txt
+./main85 >> output.txt
+./main86 >> output.txt
+./main87 >> output.txt
+./main88 >> output.txt
+./main89 >> output.txt
+./main90 >> output.txt
+./main91 >> output.txt
+./main92 >> output.txt
+./main93 >> output.txt
+./main94 >> output.txt
+./main95 >> output.txt
+./main96 >> output.txt
+./main97 >> output.txt
+./main98 >> output.txt
+./main99 >> output.txt
+./main100 >> output.txt
+./main101 >> output.txt
+./main102 >> output.txt
+./main103 >> output.txt
+./main104 >> output.txt
+./main105 >> output.txt
+./main106 >> output.txt
+./main107 >> output.txt
+./main108 >> output.txt
+./main109 >> output.txt
+./main110 >> output.txt
+./main111 >> output.txt
+./main112 >> output.txt
+./main113 >> output.txt
+./main114 >> output.txt
+./main115 >> output.txt
+./main116 >> output.txt
+./main117 >> output.txt
+./main118 >> output.txt
+./main119 >> output.txt
+./main120 >> output.txt
+./main121 >> output.txt
+./main122 >> output.txt
+./main123 >> output.txt
+./main124 >> output.txt
+./main125 >> output.txt
+./main126 >> output.txt
+./main127 >> output.txt
+./main128 >> output.txt
+./main129 >> output.txt
+./main130 >> output.txt
+./main131 >> output.txt
+./main132 >> output.txt
+./main133 >> output.txt
+./main134 >> output.txt
+./main135 >> output.txt
+./main136 >> output.txt
+./main137 >> output.txt
+./main138 >> output.txt
+./main139 >> output.txt
+./main140 >> output.txt
+./main141 >> output.txt
+./main142 >> output.txt
+./main143 >> output.txt
+./main144 >> output.txt
+./main145 >> output.txt
+./main146 >> output.txt
+./main147 >> output.txt
+./main148 >> output.txt
+./main149 >> output.txt
+./main150 >> output.txt
+./main151 >> output.txt
+./main152 >> output.txt
+./main153 >> output.txt
+./main154 >> output.txt
+./main155 >> output.txt
+./main156 >> output.txt
+./main157 >> output.txt
+./main158 >> output.txt
+./main159 >> output.txt
+./main160 >> output.txt
+./main161 >> output.txt
+./main162 >> output.txt
+./main163 >> output.txt
+./main164 >> output.txt
+./main165 >> output.txt
+./main166 >> output.txt
+./main167 >> output.txt
+./main168 >> output.txt
+./main169 >> output.txt
+./main170 >> output.txt
+./main171 >> output.txt
+./main172 >> output.txt
+./main173 >> output.txt
+./main174 >> output.txt
+./main175 >> output.txt
+./main176 >> output.txt
+./main177 >> output.txt
+./main178 >> output.txt
+./main179 >> output.txt
+./main180 >> output.txt
+./main181 >> output.txt
+./main182 >> output.txt
+./main183 >> output.txt
+./main184 >> output.txt
+./main185 >> output.txt
+./main186 >> output.txt
+./main187 >> output.txt
+./main188 >> output.txt
+./main189 >> output.txt
+./main190 >> output.txt
+./main191 >> output.txt
+./main192 >> output.txt
+./main193 >> output.txt
+./main194 >> output.txt
+./main195 >> output.txt
+./main196 >> output.txt
+./main197 >> output.txt
+./main198 >> output.txt
+./main199 >> output.txt
+./main200 >> output.txt
+./main201 >> output.txt
+./main202 >> output.txt
+./main203 >> output.txt
+./main204 >> output.txt
+./main205 >> output.txt
+./main206 >> output.txt
+./main207 >> output.txt
+./main208 >> output.txt
+./main209 >> output.txt
+./main210 >> output.txt
+./main211 >> output.txt
+./main212 >> output.txt
+./main213 >> output.txt
+./main214 >> output.txt
+./main215 >> output.txt
+./main216 >> output.txt
+./main217 >> output.txt
+./main218 >> output.txt
+./main219 >> output.txt
+./main220 >> output.txt
+./main221 >> output.txt
+./main222 >> output.txt
+./main223 >> output.txt
+./main224 >> output.txt
+./main225 >> output.txt
+./main226 >> output.txt
+./main227 >> output.txt
+./main228 >> output.txt
+./main229 >> output.txt
+./main230 >> output.txt
+./main231 >> output.txt
+./main232 >> output.txt
+./main233 >> output.txt
+./main234 >> output.txt
+./main235 >> output.txt
+./main236 >> output.txt
+./main237 >> output.txt
+./main238 >> output.txt
+./main239 >> output.txt
+./main240 >> output.txt
+./main241 >> output.txt
+./main242 >> output.txt
+./main243 >> output.txt
+./main244 >> output.txt
+./main245 >> output.txt
+./main246 >> output.txt
+./main247 >> output.txt
+./main248 >> output.txt
+./main249 >> output.txt
+./main250 >> output.txt
+./main251 >> output.txt
+./main252 >> output.txt
+./main253 >> output.txt
+./main254 >> output.txt
+./main255 >> output.txt
+./main256 >> output.txt
+./main257 >> output.txt
+./main258 >> output.txt
+./main259 >> output.txt
+./main260 >> output.txt
+./main261 >> output.txt
+./main262 >> output.txt
+./main263 >> output.txt
+./main264 >> output.txt
+./main265 >> output.txt
+./main266 >> output.txt
+./main267 >> output.txt
+./main268 >> output.txt
+./main269 >> output.txt
+./main270 >> output.txt
+./main271 >> output.txt
+./main272 >> output.txt
+./main273 >> output.txt
+./main274 >> output.txt
+./main275 >> output.txt
+./main276 >> output.txt
+./main277 >> output.txt
+./main278 >> output.txt
+./main279 >> output.txt
+./main280 >> output.txt
+./main281 >> output.txt
+./main282 >> output.txt
+./main283 >> output.txt
+./main284 >> output.txt
+./main285 >> output.txt
+./main286 >> output.txt
+./main287 >> output.txt
+./main288 >> output.txt
+./main289 >> output.txt
+./main290 >> output.txt
+./main291 >> output.txt
+./main292 >> output.txt
+./main293 >> output.txt
+./main294 >> output.txt
+./main295 >> output.txt
+./main296 >> output.txt
+./main297 >> output.txt
+./main298 >> output.txt
+./main299 >> output.txt
+./main300 >> output.txt
+./main301 >> output.txt
+./main302 >> output.txt
+./main303 >> output.txt
+./main304 >> output.txt
+./main305 >> output.txt
+./main306 >> output.txt
+./main307 >> output.txt
+./main308 >> output.txt
+./main309 >> output.txt
+./main310 >> output.txt
+./main311 >> output.txt
+./main312 >> output.txt
+./main313 >> output.txt
+./main314 >> output.txt
+./main315 >> output.txt
+./main316 >> output.txt
+./main317 >> output.txt
+./main318 >> output.txt
+./main319 >> output.txt
+./main320 >> output.txt
+./main321 >> output.txt
+./main322 >> output.txt
+./main323 >> output.txt
+./main324 >> output.txt
+./main325 >> output.txt
+./main326 >> output.txt
+./main327 >> output.txt
+./main328 >> output.txt
+./main329 >> output.txt
+./main330 >> output.txt
+./main331 >> output.txt
+./main332 >> output.txt
+./main333 >> output.txt
+./main334 >> output.txt
+./main335 >> output.txt
+./main336 >> output.txt
+./main337 >> output.txt
+./main338 >> output.txt
+./main339 >> output.txt
+./main340 >> output.txt
+./main341 >> output.txt
+./main342 >> output.txt
+./main343 >> output.txt
+./main344 >> output.txt
+./main345 >> output.txt
+./main346 >> output.txt
+./main347 >> output.txt
+./main348 >> output.txt
+./main349 >> output.txt
+./main350 >> output.txt
+./main351 >> output.txt
+./main352 >> output.txt
+./main353 >> output.txt
+./main354 >> output.txt
+./main355 >> output.txt
+./main356 >> output.txt
+./main357 >> output.txt
+./main358 >> output.txt
+./main359 >> output.txt
+./main360 >> output.txt
+./main361 >> output.txt
+./main362 >> output.txt
+./main363 >> output.txt
+./main364 >> output.txt
+./main365 >> output.txt
+./main366 >> output.txt
+./main367 >> output.txt
+./main368 >> output.txt
+./main369 >> output.txt
+./main370 >> output.txt
+./main371 >> output.txt
+./main372 >> output.txt
+./main373 >> output.txt
+./main374 >> output.txt
+./main375 >> output.txt
+./main376 >> output.txt
+./main377 >> output.txt
+./main378 >> output.txt
+./main379 >> output.txt
+./main380 >> output.txt
+./main381 >> output.txt
+./main382 >> output.txt
+./main383 >> output.txt
+./main384 >> output.txt
+./main385 >> output.txt
+./main386 >> output.txt
+./main387 >> output.txt
+./main388 >> output.txt
+./main389 >> output.txt
+./main390 >> output.txt
+./main391 >> output.txt
+./main392 >> output.txt
+./main393 >> output.txt
+./main394 >> output.txt
+./main395 >> output.txt
+./main396 >> output.txt
+./main397 >> output.txt
+./main398 >> output.txt
+./main399 >> output.txt
+./main400 >> output.txt
+./main401 >> output.txt
+./main402 >> output.txt
+./main403 >> output.txt
+./main404 >> output.txt
+./main405 >> output.txt
+./main406 >> output.txt
+./main407 >> output.txt
+./main408 >> output.txt
+./main409 >> output.txt
+./main410 >> output.txt
+./main411 >> output.txt
+./main412 >> output.txt
+./main413 >> output.txt
+./main414 >> output.txt
+./main415 >> output.txt
+./main416 >> output.txt
+./main417 >> output.txt
+./main418 >> output.txt
+./main419 >> output.txt
+./main420 >> output.txt
+./main421 >> output.txt
+./main422 >> output.txt
+./main423 >> output.txt
+./main424 >> output.txt
+./main425 >> output.txt
+./main426 >> output.txt
+./main427 >> output.txt
+./main428 >> output.txt
+./main429 >> output.txt
+./main430 >> output.txt
+./main431 >> output.txt
+./main432 >> output.txt
+./main433 >> output.txt
+./main434 >> output.txt
+./main435 >> output.txt
+./main436 >> output.txt
+./main437 >> output.txt
+./main438 >> output.txt
+./main439 >> output.txt
+./main440 >> output.txt
+./main441 >> output.txt
+./main442 >> output.txt
+./main443 >> output.txt
+./main444 >> output.txt
+./main445 >> output.txt
+./main446 >> output.txt
+./main447 >> output.txt
+./main448 >> output.txt
+./main449 >> output.txt
+./main450 >> output.txt
+./main451 >> output.txt
+./main452 >> output.txt
+./main453 >> output.txt
+./main454 >> output.txt
+./main455 >> output.txt
+./main456 >> output.txt
+./main457 >> output.txt
+./main458 >> output.txt
+./main459 >> output.txt
+./main460 >> output.txt
+./main461 >> output.txt
+./main462 >> output.txt
+./main463 >> output.txt
+./main464 >> output.txt
+./main465 >> output.txt
+./main466 >> output.txt
+./main467 >> output.txt
+./main468 >> output.txt
+./main469 >> output.txt
+./main470 >> output.txt
+./main471 >> output.txt
+./main472 >> output.txt
+./main473 >> output.txt
+./main474 >> output.txt
+./main475 >> output.txt
+./main476 >> output.txt
+./main477 >> output.txt
+./main478 >> output.txt
+./main479 >> output.txt
+./main480 >> output.txt
+./main481 >> output.txt
+./main482 >> output.txt
+./main483 >> output.txt
+./main484 >> output.txt
+./main485 >> output.txt
+./main486 >> output.txt
+./main487 >> output.txt
+./main488 >> output.txt
+./main489 >> output.txt
+./main490 >> output.txt
+./main491 >> output.txt
+./main492 >> output.txt
+./main493 >> output.txt
+./main494 >> output.txt
+./main495 >> output.txt
+./main496 >> output.txt
+./main497 >> output.txt
+./main498 >> output.txt
+./main499 >> output.txt
+./main500 >> output.txt
+./main501 >> output.txt
+./main502 >> output.txt
+./main503 >> output.txt
+./main504 >> output.txt
+./main505 >> output.txt
+./main506 >> output.txt
+./main507 >> output.txt
+./main508 >> output.txt
+./main509 >> output.txt
+./main510 >> output.txt
+./main511 >> output.txt
+./main512 >> output.txt
+./main513 >> output.txt
+./main514 >> output.txt
+./main515 >> output.txt
+./main516 >> output.txt
+./main517 >> output.txt
+./main518 >> output.txt
+./main519 >> output.txt
+./main520 >> output.txt
+./main521 >> output.txt
+./main522 >> output.txt
+./main523 >> output.txt
+./main524 >> output.txt
+./main525 >> output.txt
+./main526 >> output.txt
+./main527 >> output.txt
+./main528 >> output.txt
+./main529 >> output.txt
+./main530 >> output.txt
+./main531 >> output.txt
+./main532 >> output.txt
+./main533 >> output.txt
+./main534 >> output.txt
+./main535 >> output.txt
+./main536 >> output.txt
+./main537 >> output.txt
+./main538 >> output.txt
+./main539 >> output.txt
+./main540 >> output.txt
+./main541 >> output.txt
+./main542 >> output.txt
+./main543 >> output.txt
+./main544 >> output.txt
+./main545 >> output.txt
+./main546 >> output.txt
+./main547 >> output.txt
+./main548 >> output.txt
+./main549 >> output.txt
+./main550 >> output.txt
+./main551 >> output.txt
+./main552 >> output.txt
+./main553 >> output.txt
+./main554 >> output.txt
+./main555 >> output.txt
+./main556 >> output.txt
+./main557 >> output.txt
+./main558 >> output.txt
+./main559 >> output.txt
+./main560 >> output.txt
+./main561 >> output.txt
+./main562 >> output.txt
+./main563 >> output.txt
+./main564 >> output.txt
+./main565 >> output.txt
+./main566 >> output.txt
+./main567 >> output.txt
+./main568 >> output.txt
+./main569 >> output.txt
+./main570 >> output.txt
+./main571 >> output.txt
+./main572 >> output.txt
+./main573 >> output.txt
+./main574 >> output.txt
+./main575 >> output.txt
+./main576 >> output.txt
+./main577 >> output.txt
+./main578 >> output.txt
+./main579 >> output.txt
+./main580 >> output.txt
+./main581 >> output.txt
+./main582 >> output.txt
+./main583 >> output.txt
+./main584 >> output.txt
+./main585 >> output.txt
+./main586 >> output.txt
+./main587 >> output.txt
+./main588 >> output.txt
+./main589 >> output.txt
+./main590 >> output.txt
+./main591 >> output.txt
+./main592 >> output.txt
+./main593 >> output.txt
+./main594 >> output.txt
+./main595 >> output.txt
+./main596 >> output.txt
+./main597 >> output.txt
+./main598 >> output.txt
+./main599 >> output.txt
+./main600 >> output.txt
+./main601 >> output.txt
+./main602 >> output.txt
+./main603 >> output.txt
+./main604 >> output.txt
+./main605 >> output.txt
+./main606 >> output.txt
+./main607 >> output.txt
+./main608 >> output.txt
+./main609 >> output.txt
+./main610 >> output.txt
+./main611 >> output.txt
+./main612 >> output.txt
+./main613 >> output.txt
+./main614 >> output.txt
+./main615 >> output.txt
+./main616 >> output.txt
+./main617 >> output.txt
+./main618 >> output.txt
+./main619 >> output.txt
+./main620 >> output.txt
+./main621 >> output.txt
+./main622 >> output.txt
+./main623 >> output.txt
+./main624 >> output.txt
+./main625 >> output.txt
+./main626 >> output.txt
+./main627 >> output.txt
+./main628 >> output.txt
+./main629 >> output.txt
+./main630 >> output.txt
+./main631 >> output.txt
+./main632 >> output.txt
+./main633 >> output.txt
+./main634 >> output.txt
+./main635 >> output.txt
+./main636 >> output.txt
+./main637 >> output.txt
+./main638 >> output.txt
+./main639 >> output.txt
+./main640 >> output.txt
+./main641 >> output.txt
+./main642 >> output.txt
+./main643 >> output.txt
+./main644 >> output.txt
+./main645 >> output.txt
+./main646 >> output.txt
+./main647 >> output.txt
+./main648 >> output.txt
+./main649 >> output.txt
+./main650 >> output.txt
+./main651 >> output.txt
+./main652 >> output.txt
+./main653 >> output.txt
+./main654 >> output.txt
+./main655 >> output.txt
+./main656 >> output.txt
+./main657 >> output.txt
+./main658 >> output.txt
+./main659 >> output.txt
+./main660 >> output.txt
+./main661 >> output.txt
+./main662 >> output.txt
+./main663 >> output.txt
+./main664 >> output.txt
+./main665 >> output.txt
+./main666 >> output.txt
+./main667 >> output.txt
+./main668 >> output.txt
+./main669 >> output.txt
+./main670 >> output.txt
+./main671 >> output.txt
+./main672 >> output.txt
+./main673 >> output.txt
+./main674 >> output.txt
+./main675 >> output.txt
+./main676 >> output.txt
+./main677 >> output.txt
+./main678 >> output.txt
+./main679 >> output.txt
+./main680 >> output.txt
+./main681 >> output.txt
+./main682 >> output.txt
+./main683 >> output.txt
+./main684 >> output.txt
+./main685 >> output.txt
+./main686 >> output.txt
+./main687 >> output.txt
+./main688 >> output.txt
+./main689 >> output.txt
+./main690 >> output.txt
+./main691 >> output.txt
+./main692 >> output.txt
+./main693 >> output.txt
+./main694 >> output.txt
+./main695 >> output.txt
+./main696 >> output.txt
+./main697 >> output.txt
+./main698 >> output.txt
+./main699 >> output.txt
+./main700 >> output.txt
+./main701 >> output.txt
+./main702 >> output.txt
+./main703 >> output.txt
+./main704 >> output.txt
+./main705 >> output.txt
+./main706 >> output.txt
+./main707 >> output.txt
+./main708 >> output.txt
+./main709 >> output.txt
+./main710 >> output.txt
+./main711 >> output.txt
+./main712 >> output.txt
+./main713 >> output.txt
+./main714 >> output.txt
+./main715 >> output.txt
+./main716 >> output.txt
+./main717 >> output.txt
+./main718 >> output.txt
+./main719 >> output.txt
+./main720 >> output.txt
+./main721 >> output.txt
+./main722 >> output.txt
+./main723 >> output.txt
+./main724 >> output.txt
+./main725 >> output.txt
+./main726 >> output.txt
+./main727 >> output.txt
+./main728 >> output.txt
+./main729 >> output.txt
+./main730 >> output.txt
+./main731 >> output.txt
+./main732 >> output.txt
+./main733 >> output.txt
+./main734 >> output.txt
+./main735 >> output.txt
+./main736 >> output.txt
+./main737 >> output.txt
+./main738 >> output.txt
+./main739 >> output.txt
+./main740 >> output.txt
+./main741 >> output.txt
+./main742 >> output.txt
+./main743 >> output.txt
+./main744 >> output.txt
+./main745 >> output.txt
+./main746 >> output.txt
+./main747 >> output.txt
+./main748 >> output.txt
+./main749 >> output.txt
+./main750 >> output.txt
+./main751 >> output.txt
+./main752 >> output.txt
+./main753 >> output.txt
+./main754 >> output.txt
+./main755 >> output.txt
+./main756 >> output.txt
+./main757 >> output.txt
+./main758 >> output.txt
+./main759 >> output.txt
+./main760 >> output.txt
+./main761 >> output.txt
+./main762 >> output.txt
+./main763 >> output.txt
+./main764 >> output.txt
+./main765 >> output.txt
+./main766 >> output.txt
+./main767 >> output.txt
+./main768 >> output.txt
+./main769 >> output.txt
+./main770 >> output.txt
+./main771 >> output.txt
+./main772 >> output.txt
+./main773 >> output.txt
+./main774 >> output.txt
+./main775 >> output.txt
+./main776 >> output.txt
+./main777 >> output.txt
+./main778 >> output.txt
+./main779 >> output.txt
+./main780 >> output.txt
+./main781 >> output.txt
+./main782 >> output.txt
+./main783 >> output.txt
+./main784 >> output.txt
+./main785 >> output.txt
+./main786 >> output.txt
+./main787 >> output.txt
+./main788 >> output.txt
+./main789 >> output.txt
+./main790 >> output.txt
+./main791 >> output.txt
+./main792 >> output.txt
+./main793 >> output.txt
+./main794 >> output.txt
+./main795 >> output.txt
+./main796 >> output.txt
+./main797 >> output.txt
+./main798 >> output.txt
+./main799 >> output.txt
+./main800 >> output.txt
+./main801 >> output.txt
+./main802 >> output.txt
+./main803 >> output.txt
+./main804 >> output.txt
+./main805 >> output.txt
+./main806 >> output.txt
+./main807 >> output.txt
+./main808 >> output.txt
+./main809 >> output.txt
+./main810 >> output.txt
+./main811 >> output.txt
+./main812 >> output.txt
+./main813 >> output.txt
+./main814 >> output.txt
+./main815 >> output.txt
+./main816 >> output.txt
+./main817 >> output.txt
+./main818 >> output.txt
+./main819 >> output.txt
+./main820 >> output.txt
+./main821 >> output.txt
+./main822 >> output.txt
+./main823 >> output.txt
+./main824 >> output.txt
+./main825 >> output.txt
+./main826 >> output.txt
+./main827 >> output.txt
+./main828 >> output.txt
+./main829 >> output.txt
+./main830 >> output.txt
+./main831 >> output.txt
+./main832 >> output.txt
+./main833 >> output.txt
+./main834 >> output.txt
+./main835 >> output.txt
+./main836 >> output.txt
+./main837 >> output.txt
+./main838 >> output.txt
+./main839 >> output.txt
+./main840 >> output.txt
+./main841 >> output.txt
+./main842 >> output.txt
+./main843 >> output.txt
+./main844 >> output.txt
+./main845 >> output.txt
+./main846 >> output.txt
+./main847 >> output.txt
+./main848 >> output.txt
+./main849 >> output.txt
+./main850 >> output.txt
+./main851 >> output.txt
+./main852 >> output.txt
+./main853 >> output.txt
+./main854 >> output.txt
+./main855 >> output.txt
+./main856 >> output.txt
+./main857 >> output.txt
+./main858 >> output.txt
+./main859 >> output.txt
+./main860 >> output.txt
+./main861 >> output.txt
+./main862 >> output.txt
+./main863 >> output.txt
+./main864 >> output.txt
+./main865 >> output.txt
+./main866 >> output.txt
+./main867 >> output.txt
+./main868 >> output.txt
+./main869 >> output.txt
+./main870 >> output.txt
+./main871 >> output.txt
+./main872 >> output.txt
+./main873 >> output.txt
+./main874 >> output.txt
+./main875 >> output.txt
+./main876 >> output.txt
+./main877 >> output.txt
+./main878 >> output.txt
+./main879 >> output.txt
+./main880 >> output.txt
+./main881 >> output.txt
+./main882 >> output.txt
+./main883 >> output.txt
+./main884 >> output.txt
+./main885 >> output.txt
+./main886 >> output.txt
+./main887 >> output.txt
+./main888 >> output.txt
+./main889 >> output.txt
+./main890 >> output.txt
+./main891 >> output.txt
+./main892 >> output.txt
+./main893 >> output.txt
+./main894 >> output.txt
+./main895 >> output.txt
+./main896 >> output.txt
+./main897 >> output.txt
+./main898 >> output.txt
+./main899 >> output.txt
+./main900 >> output.txt
+./main901 >> output.txt
+./main902 >> output.txt
+./main903 >> output.txt
+./main904 >> output.txt
+./main905 >> output.txt
+./main906 >> output.txt
+./main907 >> output.txt
+./main908 >> output.txt
+./main909 >> output.txt
+./main910 >> output.txt
+./main911 >> output.txt
+./main912 >> output.txt
+./main913 >> output.txt
+./main914 >> output.txt
+./main915 >> output.txt
+./main916 >> output.txt
+./main917 >> output.txt
+./main918 >> output.txt
+./main919 >> output.txt
+./main920 >> output.txt
+./main921 >> output.txt
+./main922 >> output.txt
+./main923 >> output.txt
+./main924 >> output.txt
+./main925 >> output.txt
+./main926 >> output.txt
+./main927 >> output.txt
+./main928 >> output.txt
+./main929 >> output.txt
+./main930 >> output.txt
+./main931 >> output.txt
+./main932 >> output.txt
+./main933 >> output.txt
+./main934 >> output.txt
+./main935 >> output.txt
+./main936 >> output.txt
+./main937 >> output.txt
+./main938 >> output.txt
+./main939 >> output.txt
+./main940 >> output.txt
+./main941 >> output.txt
+./main942 >> output.txt
+./main943 >> output.txt
+./main944 >> output.txt
+./main945 >> output.txt
+./main946 >> output.txt
+./main947 >> output.txt
+./main948 >> output.txt
+./main949 >> output.txt
+./main950 >> output.txt
+./main951 >> output.txt
+./main952 >> output.txt
+./main953 >> output.txt
+./main954 >> output.txt
+./main955 >> output.txt
+./main956 >> output.txt
+./main957 >> output.txt
+./main958 >> output.txt
+./main959 >> output.txt
+./main960 >> output.txt
+./main961 >> output.txt
+./main962 >> output.txt
+./main963 >> output.txt
+./main964 >> output.txt
+./main965 >> output.txt
+./main966 >> output.txt
+./main967 >> output.txt
+./main968 >> output.txt
+./main969 >> output.txt
+./main970 >> output.txt
+./main971 >> output.txt
+./main972 >> output.txt
+./main973 >> output.txt
+./main974 >> output.txt
+./main975 >> output.txt
+date +%s ;
